quotation/theories/ToPCUIC/QuotationOf/Common/Universes/ConstraintSetExtraDecide/Instances.v
@@ -2,6 +2,6 @@ From MetaRocq.Common Require Import Universes.
 From MetaRocq.Quotation.ToPCUIC Require Import Init.
 From MetaRocq.Quotation.ToPCUIC.QuotationOf.Utils Require Import MRMSets.Sig.
 
-Module qConstraintSetExtraDecide <: MSetAVL.QuotationOfDecide UnivConstraintSet.E UnivConstraintSet UnivConstraintSetExtraDecide.
+Module qUnivConstraintSetExtraDecide <: MSetAVL.QuotationOfDecide UnivConstraintSet.E UnivConstraintSet UnivConstraintSetExtraDecide.
   MetaRocq Run (tmMakeQuotationOfModule everything None "UnivConstraintSetExtraDecide").
-End qConstraintSetExtraDecide.
+End qUnivConstraintSetExtraDecide.
